devel/Iron/Language/SystemF2Effect/Step.v
@@ -8,79 +8,85 @@ Require Export Iron.Language.SystemF2Effect.Value.
 (** The single step rules model the individual transitions that the 
      machine can make at runtime. *)
 
-Inductive STEP : store -> exp -> store -> exp -> Prop :=
+Inductive 
+  STEP :  store -> stprops -> exp 
+       -> store -> stprops -> exp 
+       -> Prop :=
 
  (* Step an expression in the let context. *)
  | EsLet 
-   :  forall t s x1 x2 s' x1'
-   ,  STEP s x1             s' x1'
-   -> STEP s  (XLet t x1 x2) 
-           s' (XLet t x1' x2)
+   :  forall ss sp ss' sp' t x1 x1' x2
+   ,  STEP ss sp x1 ss' sp' x1'
+   -> STEP ss  sp   (XLet t x1  x2) 
+           ss' sp'  (XLet t x1' x2)
 
  (* Let substitution. *)
  | EsLetSubst
-   :  forall t s v x2
-   ,  STEP s (XLet t (XVal v) x2) 
-           s (substVX 0 v x2)
+   :  forall ss sp t v x2
+   ,  STEP ss sp    (XLet t (XVal v) x2) 
+           ss sp    (substVX 0 v x2)
 
  (* Value application. *)
  | EsAppSubst
-   : forall s t11 x12 v2
-   ,  STEP s (XApp (VLam t11 x12) v2)
-           s (substVX 0 v2 x12)
+   :  forall ss sp t11 x12 v2
+   ,  STEP ss sp    (XApp (VLam t11 x12) v2)
+           ss sp    (substVX 0 v2 x12)
 
  (* Type application. *)
  | EsLAMSubst
-   :  forall s k11 x12 t2      
-   ,  STEP s (XAPP (VLAM k11 x12) t2)
-           s (substTX 0 t2 x12)
+   :  forall ss sp k11 x12 t2      
+   ,  STEP ss sp    (XAPP (VLAM k11 x12) t2)
+           ss sp    (substTX 0 t2 x12)
 
  (* Create a new region. *)
  | EsNew
-   :  forall s x
-   ,  STEP s                   (XNew x) 
-           (SDesc <: s)        (substTX 0 (TCon (TyConRegion (length s))) x)
+   :  forall ss sp x
+   ,  STEP ss sp              (XNew x) 
+           ss (SRegion <: sp) (substTX 0 (TCon (TyConRegion (length sp))) x)
 
  (* Evaluation with a region. *)
  | EsUse
-   :  forall n s s' x x'
-   ,  STEP s x s' x'
-   -> STEP s (XUse n x) s' (XUse n x')
+   :  forall ss sp ss' sp' x x' n
+   ,  STEP ss sp x ss' sp' x'
+   -> STEP ss  sp   (XUse n x) 
+           ss' sp'  (XUse n x')
 
  (* Pop a region from the stack. *)
  | EsUsePop
-   :  forall s n v
-   ,  STEP s (XUse n (XVal v)) s (XVal v)
+   :  forall ss sp n v
+   ,  STEP ss  sp   (XUse n (XVal v)) 
+           ss  sp   (XVal v)
 
  (* Allocate a reference. *) 
  | EsAlloc
-   :  forall s r1 v1
-   ,  STEP s                   (XAlloc (TCon (TyConRegion r1)) v1)
-           (SValue r1 v1 <: s) (XVal (VLoc (length s)))
+   :  forall ss sp r1 v1
+   ,  STEP ss                    sp (XAlloc (TCon (TyConRegion r1)) v1)
+           (StValue r1 v1 <: ss) sp (XVal (VLoc (length ss)))
 
  (* Read from a reference. *)
  | EsRead
-   :  forall s l v r
-   ,  get l s = Some (SValue r v)
-   -> STEP s (XRead (TCon (TyConRegion r)) (VLoc l)) s (XVal v)
+   :  forall ss sp l v r
+   ,  get l ss = Some (StValue r v)
+   -> STEP ss sp    (XRead (TCon (TyConRegion r)) (VLoc l)) 
+           ss sp    (XVal v)
 
  (* Write to a reference. *)
  | EsWrite 
-   :  forall s l r v
-   ,  STEP s    (XWrite (TCon (TyConRegion r)) (VLoc l) v)
-           (update l (SValue r v) s) (XVal (VConst CUnit))
+   :  forall ss sp l r v
+   ,  STEP ss sp    (XWrite (TCon (TyConRegion r)) (VLoc l) v)
+           (update l (StValue r v) ss) sp (XVal (VConst CUnit))
 
  (* Take the successor of a natural. *)
  | EsSucc
-   :  forall s n
-   ,  STEP s  (XOp1 OSucc (VConst (CNat n)))
-           s  (XVal (VConst (CNat (S n))))
+   :  forall ss sp n
+   ,  STEP ss sp    (XOp1 OSucc (VConst (CNat n)))
+           ss sp    (XVal (VConst (CNat (S n))))
 
  (* Test a natural for zero. *)
  | EsIsZeroTrue 
-   :  forall s n
-   ,  STEP s  (XOp1 OIsZero (VConst (CNat n)))
-           s  (XVal (VConst (CBool (beq_nat n 0)))).
+   :  forall ss sp n
+   ,  STEP ss sp    (XOp1 OIsZero (VConst (CNat n)))
+           ss sp    (XVal (VConst (CBool (beq_nat n 0)))).
 
 Hint Constructors STEP.
 
