devel/Iron/Language/SystemF2Effect/Store/Bind.v
@@ -4,20 +4,16 @@ Require Export Iron.Language.SystemF2Effect.Value.
 
 (* Store bindings are the primitive objects we keep in the store.
    Each one is tagged with the number of the region is in. *)
-Inductive sbind :=
- (* A region descriptor.
-    One of these exists in the store for every live region. *)
- | SDesc  : sbind
-
+Inductive stbind :=
  (* A store value in some region. *)
- | SValue : nat -> val -> sbind.
+ | StValue : nat -> val -> stbind.
 
-Hint Constructors sbind.
+Hint Constructors stbind.
 
 
 (* Types of store bindings. *)
-Inductive TYPEB : kienv -> tyenv -> stenv -> sbind -> ty -> Prop := 
+Inductive TYPEB : kienv -> tyenv -> stenv -> stprops -> stbind -> ty -> Prop := 
  | TbValue
-   :  forall ke te se n v t
-   ,  TYPEV ke te se v t
-   -> TYPEB ke te se (SValue n v) (tRef (TCon (TyConRegion n)) t).
+   :  forall ke te se sp n v t
+   ,  TYPEV  ke te se sp v t
+   -> TYPEB  ke te se sp (StValue n v) (tRef (TCon (TyConRegion n)) t).
