devel/Iron/Language/SystemF2Effect/Store/Prop.v
@@ -1,0 +1,10 @@
+
+
+
+Inductive stprop :=
+ (* A region descriptor.
+    One of these exists in the store for every live region in the store. *)
+ | SRegion  : stprop.
+
+
+Definition stprops := list stprop.
