devel/Iron/Language/SystemF2Effect/Value/TyJudge/Unique.v
@@ -2,61 +2,63 @@
 Require Import Iron.Language.SystemF2Effect.Value.TyJudge.
 
 
-(* Uniqueness of typing *)
-Lemma type_unique
- :  forall ke te se x t1 e1 t2 e2
- ,  TYPEX ke te se x t1 e1
- -> TYPEX ke te se x t2 e2
+(* Uniqueness of typing.
+   Checking an expression always returns a unique type an effect. *)
+Lemma typex_unique
+ :  forall ke te se sp x t1 e1 t2 e2
+ ,  TYPEX  ke te se sp x t1 e1
+ -> TYPEX  ke te se sp x t2 e2
  -> t1 = t2 /\ e1 = e2.
 Proof.
- intros. gen ke te se t1 e1 t2 e2.
+ intros. gen ke te se sp t1 e1 t2 e2.
  induction x using exp_mutind with 
-  (PV := fun v1 => forall ke te se t1 t1'
-      ,  TYPEV ke te se v1 t1
-      -> TYPEV ke te se v1 t1'
+  (PV := fun v1 => forall ke te se sp t1 t1'
+      ,  TYPEV ke te se sp v1 t1
+      -> TYPEV ke te se sp v1 t1'
       -> t1 = t1');
   intros; 
    try (solve [inverts_type; try congruence]);
    inverts_type; auto.
 
  Case "VLam".
-  spec IHx H8 H9. burn.
+  spec IHx H9 H10. 
+  burn.
 
  Case "VLAM".
-  spec IHx H7 H6. burn.
+  spec IHx H8 H7.
+  burn.
 
  Case "XVal".
-  spec IHx H5 H4. burn.
+  spec IHx H6 H5.
+  burn.
 
  Case "XLet".
-  spec IHx1 H10 H12.
-  spec IHx2 H11 H13. 
+  spec IHx1 H11 H13.
+  spec IHx2 H12 H14. 
   rip.
 
  Case "XApp".
-  spec IHx  H6 H5.
-  spec IHx0 H9 H10.
-  subst.
-  inverts IHx. auto.
+  spec IHx  H7  H6.
+  spec IHx0 H10 H11.
+  subst. inverts IHx. auto.
 
  Case "VAPP". 
-  spec IHx H6 H5.
-  inverts IHx.
-  auto.
+  spec IHx H7 H6.
+  inverts IHx. auto.
 
  Case "XNew".
-  spec IHx H7 H9.
+  spec IHx H8 H10.
   rip.
 
  Case "XUse".
-  spec IHx H8 H7.
+  spec IHx H9 H8.
   rip.
 
  Case "XAlloc".
-  spec IHx H9 H10.
+  spec IHx H10 H11.
   subst. burn.
 
  Case "XRead".
-  spec IHx H9 H10.
+  spec IHx H10 H11.
   inverts IHx. auto.
 Qed.
