devel/Iron/Language/SystemF2Effect/Value/TyJudge/WeakKiEnv.v
@@ -4,16 +4,16 @@ Require Import Iron.Language.SystemF2Effect.Value.TyJudge.
 
 (* Weakening Kind Env in Type Judgement. *)
 Lemma type_kienv_insert
- :  forall ix ke te se x1 t1 e1 k2
- ,  TYPEX ke te se x1 t1 e1
- -> TYPEX (insert ix k2 ke) (liftTE ix te)   (liftTE ix se) 
+ :  forall ke te se sp x1 t1 e1 k2 ix
+ ,  TYPEX  ke te se sp x1 t1 e1
+ -> TYPEX (insert ix k2 ke) (liftTE ix te)   (liftTE ix se)   sp
           (liftTX ix x1)    (liftTT 1 ix t1) (liftTT 1 ix e1).
 Proof.
- intros. gen ix ke te se t1 e1 k2.
+ intros. gen ix ke te se sp t1 e1 k2.
  induction x1 using exp_mutind with 
-  (PV := fun v => forall ix ke te se k2 t3
-               ,  TYPEV ke te se v t3
-               -> TYPEV (insert ix k2 ke) (liftTE ix te)   (liftTE ix se)
+  (PV := fun v => forall ix ke te se sp k2 t3
+               ,  TYPEV ke te se sp v t3
+               -> TYPEV (insert ix k2 ke) (liftTE ix te)   (liftTE ix se) sp
                         (liftTV ix v)     (liftTT 1 ix t3));
    intros; inverts_type; simpl; eauto.
 
@@ -32,7 +32,7 @@ Proof.
    apply kind_kienv_insert. auto.
    rrwrite ( liftTE ix te :> liftTT 1 ix t
            = liftTE ix (te :> t)).
-   spec IHx1 H7.
+   spec IHx1 H8.
    burn.
 
  Case "VLAM".
@@ -53,21 +53,21 @@ Proof.
 
  Case "XApp".
   eapply TxApp.
-   eapply IHx1 in H5. simpl in H5. eauto.
-   eapply IHx0 in H8. eauto.
+   eapply IHx1 in H6. simpl in H6. eauto.
+   eapply IHx0 in H9. eauto.
 
  Case "XAPP".
   rewrite (liftTT_substTT' 0 ix). 
   simpl.
   eapply TvAPP.
-  eapply (IHx1 ix) in H5. simpl in H5. eauto.
+  eapply (IHx1 ix) in H6. simpl in H6. eauto.
   auto using kind_kienv_insert.
 
  Case "XNew".
   eapply TxNew 
    with (t := liftTT 1 (S ix) t)
         (e := liftTT 1 (S ix) e).
-  admit. admit.                    (* looks reasonable *)
+  admit. admit.                      (* ok, lowerTT_liftTT *)
   rewrite insert_rewind.
   rewrite (liftTE_liftTE 0 ix).
   rewrite (liftTE_liftTE 0 ix).
@@ -84,19 +84,19 @@ Proof.
 
  Case "XWrite".
   eapply TxOpWrite; eauto using kind_kienv_insert.
-  eapply IHx1 in H9. simpl in H9. eauto.
-  eapply IHx1 in H7. eauto.
+  eapply IHx1 in H10. simpl in H10. eauto.
+  eapply IHx1 in H8. eauto.
 
  Case "XIsZero".
   eapply TxOpIsZero.
-  eapply IHx1 in H7. eauto.
+  eapply IHx1 in H8. eauto.
 Qed.
 
 
 Lemma type_kienv_weaken1
- :  forall ke te se x1 t1 e1 k2
- ,  TYPEX ke te se x1 t1 e1
- -> TYPEX (ke :> k2)    (liftTE 0 te)   (liftTE 0 se) 
+ :  forall ke te se sp x1 t1 e1 k2
+ ,  TYPEX  ke te se sp x1 t1 e1
+ -> TYPEX (ke :> k2)    (liftTE 0 te)   (liftTE 0 se)   sp
           (liftTX 0 x1) (liftTT 1 0 t1) (liftTT 1 0 e1).
 Proof.
  intros.
@@ -108,14 +108,15 @@ Qed.
 
 
 Lemma typev_kienv_weaken1
- :  forall ke te se v1 t1 k2
- ,  TYPEV  ke te se v1 t1
- -> TYPEV (ke :> k2)    (liftTE 0 te) (liftTE 0 se)
+ :  forall ke te se sp v1 t1 k2
+ ,  TYPEV  ke te se sp v1 t1
+ -> TYPEV (ke :> k2)    (liftTE 0 te) (liftTE 0 se) sp
           (liftTV 0 v1) (liftTT 1 0 t1).
 Proof.
  intros.
- have HX: (TYPEX ke te se (XVal v1) t1 (TBot KEffect)).
+ have HX: (TYPEX ke te se sp (XVal v1) t1 (TBot KEffect)).
  eapply type_kienv_weaken1 in HX.
  simpl in HX.
  inverts HX. eauto.
 Qed.
+
