devel/Iron/Language/SystemF2Effect/Value/TyJudge/WeakStEnv.v
@@ -4,22 +4,22 @@ Require Import Iron.Language.SystemF2Effect.Value.TyJudge.
 
 (* Weakening Store Typing in Type Judgement. *)
 Lemma typex_stenv_snoc 
- :  forall ke te se t2 x t1 e1
+ :  forall ke te se sp t2 x t1 e1
  ,  closedT t2
- -> TYPEX ke te se         x t1 e1
- -> TYPEX ke te (t2 <: se) x t1 e1.
+ -> TYPEX  ke te se         sp x t1 e1
+ -> TYPEX  ke te (t2 <: se) sp x t1 e1.
 Proof.
- intros. gen ke te se t1 e1 t2.
+ intros. gen ke te se sp t1 e1 t2.
  induction x using exp_mutind with 
-  (PV := fun v => forall ke te se t1 t2
+  (PV := fun v => forall ke te se sp t1 t2
       ,  closedT t2
-      -> TYPEV ke te se         v t1
-      -> TYPEV ke te (t2 <: se) v t1)
+      -> TYPEV ke te se         sp v t1
+      -> TYPEV ke te (t2 <: se) sp v t1)
   ; intros; inverts_type; eauto.
 
  Case "VLAM".
   eapply TvLAM.
-  spec IHx H7 H. clear H7.
+  spec IHx H8 H. clear H8.
   unfold liftTE in *.
   simpl. norm. 
   rrwrite (liftTT 1 0 t2 = t2).
@@ -27,7 +27,7 @@ Proof.
 
  Case "XNew".
   eapply TxNew with (t := t) (e := e); eauto.
-  spec IHx H7 H. clear H7.
+  spec IHx H8 H. clear H8.
   unfold liftTE in *.
   simpl. norm.
   rrwrite (liftTT 1 0 t2 = t2).
@@ -37,12 +37,12 @@ Hint Resolve typex_stenv_snoc.
 
 
 Lemma typex_stenv_weaken
- :  forall ke te se1 se2 x t1 e1
+ :  forall ke te se1 se2 sp x t1 e1
  ,  Forall closedT se2
- -> TYPEX  ke te  se1         x t1 e1
- -> TYPEX  ke te (se2 >< se1) x t1 e1.
+ -> TYPEX  ke te  se1         sp x t1 e1
+ -> TYPEX  ke te (se2 >< se1) sp x t1 e1.
 Proof.
- intros. gen ke te se1.
+ intros. gen ke te se1 sp.
  induction se2; intros.
   burn.
   rrwrite ((se2 :> a) >< se1 = se2 >< (a <: se1)).
@@ -52,11 +52,11 @@ Hint Resolve typex_stenv_weaken.
 
 
 Lemma typex_stenv_extends
- :  forall ke te se1 se2 x t1 e1
+ :  forall ke te se1 se2 sp x t1 e1
  ,  Forall closedT se2
  -> extends se2 se1
- -> TYPEX ke te se1 x t1 e1
- -> TYPEX ke te se2 x t1 e1.
+ -> TYPEX ke te se1 sp x t1 e1
+ -> TYPEX ke te se2 sp x t1 e1.
 Proof.
  intros.
  unfold extends in *.
@@ -68,17 +68,19 @@ Hint Resolve typex_stenv_extends.
 
 
 Lemma typev_stenv_extends
- :  forall ke te se1 se2 v t1
+ :  forall ke te sp se1 se2 v t1
  ,  Forall closedT se2
  -> extends se2 se1
- -> TYPEV ke te se1 v t1
- -> TYPEV ke te se2 v t1.
+ -> TYPEV ke te se1 sp v t1
+ -> TYPEV ke te se2 sp v t1.
 Proof.
  intros.
  unfold extends in *.
  destruct H0 as [se3]. subst.
- assert (TYPEX ke te (se3 >< se1) (XVal v) t1 (TBot KEffect)) as HX.
+ assert (TYPEX ke te (se3 >< se1) sp (XVal v) t1 (TBot KEffect)) as HX.
   eauto.
  inverts HX. auto.
 Qed.
 Hint Resolve typex_stenv_extends.
+
+
